

AMATH 351

Homework 8

Althea Lutz

2263506

Bhavna

Problem 1

Find the general solution near $x = 0$ of the following differential equations.

(a) $8x^2y'' + 10xy' + (x - 1)y = 0$.

Let $P(x) = 8x^2$, $Q(x) = 10x$, and $R(x) = x - 1$.

$P(x)$ vanishes when $8x^2 = 0 \Rightarrow x = 0$, so $x = 0$ is a singular point.

$\lim_{x \rightarrow \infty} (x - 0) \frac{10x}{8x^2} = \lim_{x \rightarrow \infty} \frac{10x^2}{8x^2} = \lim_{x \rightarrow \infty} \frac{5}{4} \rightarrow \frac{5}{4}$, which is finite.

$\lim_{x \rightarrow \infty} (x - 0)^2 \frac{x-1}{8x^2} = \lim_{x \rightarrow \infty} \frac{x^2(x-1)}{8x^2} = \lim_{x \rightarrow \infty} \frac{x-1}{8} \rightarrow \frac{-1}{8}$, which is finite.

Thus $x = 0$ is a regular singular point and we solve the differential equation using the Frobenius Method.

The solution is of the form $y = \sum_{n=0}^{\infty} a_n x^{n+r}$ where $a_n \neq 0$.

Then, $y' = \sum_{n=0}^{\infty} (n+r) a_n x^{n+r-1}$ and $y'' = \sum_{n=0}^{\infty} (n+r)(n+r-1) a_n x^{n+r-2}$.

Substituting into the differential equation, $8x^2 \sum_{n=0}^{\infty} (n+r)(n+r-1) a_n x^{n+r-2} + 10x \sum_{n=0}^{\infty} (n+r) a_n x^{n+r-1} + (x-1) \sum_{n=0}^{\infty} a_n x^{n+r} = 0$.

Rearranging, $8 \sum_{n=0}^{\infty} (n+r)(n+r-1) a_n x^{n+r} + 10 \sum_{n=0}^{\infty} (n+r) a_n x^{n+r} + \sum_{n=0}^{\infty} a_n x^{n+r+1} - \sum_{n=0}^{\infty} a_n x^{n+r} = 0$.

Making all powers equal, $8 \sum_{n=0}^{\infty} (n+r)(n+r-1) a_n x^{n+r} + 10 \sum_{n=0}^{\infty} (n+r) a_n x^{n+r} + \sum_{n=1}^{\infty} a_{n-1} x^{n+r} - \sum_{n=0}^{\infty} a_n x^{n+r} = 0$.

Factoring, $\sum_{n=0}^{\infty} [8(n+r)(n+r-1) + 10(n+r) - 1] a_n x^{n+r} + \sum_{n=0}^{\infty} a_{n-1} x^{n+r} = 0$.

When $n = 0$, $(8r(r-1) + 10r - 1) a_0 = 0$.

Since $a_0 \neq 0$, the indicial equation is $8r(r-1) + 10r - 1 = 0 \Rightarrow 8r^2 + 2r - 1 = 0$.

By the quadratic formula, $r = \frac{-2 \pm \sqrt{4+32}}{16} = \frac{-2 \pm 6}{16} \Rightarrow r_1 = \frac{1}{4}, r_2 = -\frac{1}{2}$.

$r_1 - r_2 = \frac{3}{4}$, which is not an integer.

Thus there are two independent solutions and the general solution is of the form $y = C_1 y_1 + C_2 y_2$.

For $n \geq 1$, $[8(n+r)(n+r-1) + 10(n+r) - 1] a_n + a_{n-1} = 0$.

Thus, the recurrence relation is $a_n = \frac{-a_{n-1}}{8(n+r)(n+r-1) + 10(n+r) - 1}$.

For $r_1 = \frac{1}{4}$, $a_n = \frac{-a_{n-1}}{2n(4n+3)}$ when $n \geq 1$.

When $n = 1$, $a_1 = \frac{-a_0}{14}$.

When $n = 2$, $a_2 = \frac{a_0}{616}$.

When $n = 3$, $a_3 = \frac{-a_0}{55440}$.

Thus, $y_1(x) = x^{\frac{1}{4}} (1 - \frac{x}{14} + \frac{x^2}{616} - \frac{x^3}{55440} + \dots)$.

For $r_2 = -\frac{1}{2}$, $a_n = \frac{-a_{n-1}}{2n(4n-3)}$ when $n \geq 1$.

When $n = 1$, $a_1 = -\frac{a_0}{2}$.

When $n = 2$, $a_2 = \frac{a_0}{4}$.

When $n = 3$, $a_3 = -\frac{a_0}{2160}$.

Thus, $y_2(x) = x^{-\frac{1}{2}}(1 - \frac{x}{2} + \frac{x^2}{40} - \frac{x^3}{2160} + \dots)$.

Hence, the general solution to the differential equation is $y(x) = C_1 x^{\frac{1}{4}}(1 - \frac{x}{14} + \frac{x^2}{616} - \frac{x^3}{55440} + \dots) + C_2 x^{-\frac{1}{2}}(1 - \frac{x}{2} + \frac{x^2}{40} - \frac{x^3}{2160} + \dots)$.

(b) $x^2 y'' + (x^2 - 2x)y' + 2y = 0$.

Let $P(x) = x^2$, $Q(x) = x^2 - 2x$, and $R(x) = 2$.

$P(x)$ vanishes when $x^2 = 0 \Rightarrow x = 0$, so $x = 0$ is a singular point.

$\lim_{x \rightarrow \infty} (x - 0) \frac{x^2 - 2x}{x^2} = \lim_{x \rightarrow \infty} \frac{x^3}{x^2} - \lim_{x \rightarrow \infty} \frac{2x^2}{x^2} = \lim_{x \rightarrow \infty} x - \lim_{x \rightarrow \infty} 2 \rightarrow -2$, which is finite.

$\lim_{x \rightarrow \infty} (x - 0)^2 \frac{2}{x^2} = \lim_{x \rightarrow \infty} \frac{2x^2}{x^2} = \lim_{x \rightarrow \infty} 2 \rightarrow 2$, which is finite.

Thus $x = 0$ is a regular singular point and we solve the differential equation using the Frobenius Method.

The solution is of the form $y = \sum_{n=0}^{\infty} a_n x^{n+r}$ where $a_n \neq 0$.

Then, $y' = \sum_{n=0}^{\infty} (n+r) a_n x^{n+r-1}$ and $y'' = \sum_{n=0}^{\infty} (n+r)(n+r-1) a_n x^{n+r-2}$.

Substituting into the differential equation, $x^2 \sum_{n=0}^{\infty} (n+r)(n+r-1) a_n x^{n+r-2} + x^2 \sum_{n=0}^{\infty} (n+r) a_n x^{n+r-1} - 2x \sum_{n=0}^{\infty} (n+r) a_n x^{n+r-1} + 2 \sum_{n=0}^{\infty} a_n x^{n+r} = 0$.

Rearranging, $\sum_{n=0}^{\infty} (n+r)(n+r-1) a_n x^{n+r} + \sum_{n=0}^{\infty} (n+r) a_n x^{n+r+1} - 2 \sum_{n=0}^{\infty} (n+r) a_n x^{n+r} + 2 \sum_{n=0}^{\infty} a_n x^{n+r} = 0$.

Factoring, $\sum_{n=0}^{\infty} [(n+r)(n+r-1) - 2(n+r) + 2] a_n x^{n+r} + \sum_{n=1}^{\infty} (n+r-1) a_{n-1} x^{n+r}$.

When $n = 0$, $r(r-1) - 2r + 2 = 0 \Rightarrow (r-1)(r-2) = 0 \Rightarrow r_1 = 2, r_2 = 1$.

$r_1 - r_2 = 1$, which is a positive integer.

Thus, r_1 gives a normal Frobenius solution and r_2 leads to a breakdown in recursion and the general solution is of the form $y = C_1 y_1 + C_2 y_2$ where $y_1 = x^{r_1} \sum_{n=0}^{\infty} a_n x^n$ and $y_2 = C y_1 \ln x + x^{r_2} \sum_{n=0}^{\infty} c_n x^n$.

For $n \geq 1$, $[(n+r)(n+r-1) - 2(n+r) + 2] a_n + (n+r-1) a_{n-1} = 0$.

Thus, the recurrence relation is $a_n = \frac{-a_{n-1}}{n+r-2}$.

For $r_1 = 2$, $a_n = \frac{-a_{n-1}}{n}$.

When $n = 1$, $a_1 = -a_0$.

When $n = 2$, $a_2 = \frac{a_0}{2}$.

When $n = 3$, $a_3 = \frac{-a_0}{6}$.

Thus, $y_1(x) = x^2 e^{-x}$.

By the Wronskian property, $y_2 = y_1 \int \frac{e^{-\int (1-\frac{2}{x}) dx}}{y_1^2} dx = x^2 e^{-x} \int \frac{e^{-(x-2 \ln x)}}{(x^2 e^{-x})^2} dx = x^2 e^{-x} \int \frac{x^2 e^{-x}}{x^4 e^{-2x}} dx = x^2 e^{-x} \int^x \frac{e^t}{t^2} dt$.

Hence, the general solution to the differential equation is $y(x) = C_1 x^2 e^{-x} + C_2 x^2 e^{-x} \int^x \frac{e^t}{t^2} dt$.

(c) $x^2 y'' + x y' + x^2 y = 0$.

Let $P(x) = x^2$, $Q(x) = x$, and $R(x) = x^2$.

$P(x)$ vanishes when $x^2 = 0 \Rightarrow x = 0$, so $x = 0$ is a singular point.

$\lim_{x \rightarrow \infty} (x - 0) \frac{x}{x^2} = \lim_{x \rightarrow \infty} \frac{x^2}{x^2} = \lim_{x \rightarrow \infty} 1 \rightarrow 1$, which is finite.

$\lim_{x \rightarrow \infty} (x - 0)^2 \frac{x^2}{x^2} = \lim_{x \rightarrow \infty} \frac{x^4}{x^2} = \lim_{x \rightarrow \infty} x^2 \rightarrow 0$, which is finite.

Thus $x = 0$ is a regular singular point and we solve the differential equation using the Frobenius Method.

The solution is of the form $y = \sum_{n=0}^{\infty} a_n x^{n+r}$ where $a_n \neq 0$.

Then, $y' = \sum_{n=0}^{\infty} (n+r) a_n x^{n+r-1}$ and $y'' = \sum_{n=0}^{\infty} (n+r)(n+r-1) a_n x^{n+r-2}$.

Substituting into the differential equation, $x^2 \sum_{n=0}^{\infty} (n+r)(n+r-1) a_n x^{n+r-2} + x \sum_{n=0}^{\infty} (n+r) a_n x^{n+r-1} + x^2 \sum_{n=0}^{\infty} a_n x^{n+r} = 0$.

Rearranging, $\sum_{n=0}^{\infty} (n+r)(n+r-1) a_n x^{n+r} + \sum_{n=0}^{\infty} (n+r) a_n x^{n+r} + \sum_{n=0}^{\infty} a_n x^{n+r+2} = 0$.

Factoring, $\sum_{n=0}^{\infty} [(n+r)(n+r-1) + (n+r)] a_n x^{n+r} + \sum_{n=0}^{\infty} a_{n-2} x^{n+r} = 0$.

When $n = 0$, $r(r-1) + r = 0 \Rightarrow r^2 = 0$.

$r_1 = r_2 = r = 0$, a repeated root.

Since the indicial equation has a repeated root, the solutions are $y_1 = x^r \sum_{n=0}^{\infty} a_n x^n$ and $y_2 = y_1 \ln x + x^r \sum_{n=0}^{\infty} c_n x^n$.

By substitution, $y_1 = \sum_{n=0}^{\infty} a_n x^n$ and $y_2 = y_1 \ln x + \sum_{n=0}^{\infty} c_n x^n$.

(d) $3x^2 y'' - xy' + y = 0$.

Let $P(x) = 3x^2$, $Q(x) = -x$, and $R(x) = 1$.

$P(x)$ vanishes when $3x^2 = 0 \Rightarrow x = 0$, so $x = 0$ is a singular point.

$\lim_{x \rightarrow \infty} (x-0) \frac{-x}{3x^2} = \lim_{x \rightarrow \infty} \frac{-x^2}{3x^2} = \lim_{x \rightarrow \infty} \frac{-1}{3} \rightarrow -\frac{1}{3}$, which is finite.

$\lim_{x \rightarrow \infty} (x-0)^2 \frac{1}{3x^2} = \lim_{x \rightarrow \infty} \frac{x^2}{3x^2} = \lim_{x \rightarrow \infty} \frac{1}{3} \rightarrow \frac{1}{3}$, which is finite.

Thus $x = 0$ is a regular singular point and we solve the differential equation using the Frobenius Method.

The solution is of the form $y = \sum_{n=0}^{\infty} a_n x^{n+r}$ where $a_n \neq 0$.

Then, $y' = \sum_{n=0}^{\infty} (n+r) a_n x^{n+r-1}$ and $y'' = \sum_{n=0}^{\infty} (n+r)(n+r-1) a_n x^{n+r-2}$.

Substituting into the differential equation, $3x^2 \sum_{n=0}^{\infty} (n+r)(n+r-1) a_n x^{n+r-2} - x \sum_{n=0}^{\infty} (n+r) a_n x^{n+r-1} + \sum_{n=0}^{\infty} a_n x^{n+r} = 0$.

Rearranging, $3 \sum_{n=0}^{\infty} (n+r)(n+r-1) a_n x^{n+r} - \sum_{n=0}^{\infty} (n+r) a_n x^{n+r} + \sum_{n=0}^{\infty} a_n x^{n+r} = 0$.

Factoring, $\sum_{n=0}^{\infty} [3(n+r)(n+r-1) - (n+r) + 1] a_n x^{n+r} = 0$.

When $n = 0$, $3r(r-1) - r + 1 = 0 \Rightarrow 3r^2 - 4r + 1 = 0$.

By the quadratic formula, $r = \frac{4 \pm \sqrt{16-12}}{6} = \frac{4 \pm 2}{6} \Rightarrow r_1 = 1, r_2 = \frac{1}{3}$.

$r_1 - r_2 = \frac{2}{3}$, which is not an integer, so there are two independent Frobenius solutions.

By substitution, $y_1 = x \sum_{n=0}^{\infty} a_n x^n$ and $y_2 = x^{\frac{1}{3}} \sum_{n=0}^{\infty} b_n x^n$.

(e) $2x^2 y'' + 7x(x+1)y' - 3y = 0$.

Let $P(x) = 2x^2$, $Q(x) = 7x(x+1)$, and $R(x) = -3$.

$P(x)$ vanishes when $2x^2 = 0 \Rightarrow x = 0$, so $x = 0$ is a singular point.

$\lim_{x \rightarrow \infty} (x-0) \frac{7x^2+7x}{2x^2} = \lim_{x \rightarrow \infty} \frac{7x^3+7x^2}{2x^2} = \lim_{x \rightarrow \infty} \frac{7x+7}{2} \rightarrow \frac{7}{2}$, which is finite.

$\lim_{x \rightarrow \infty} (x-0)^2 \frac{7x^2+7x}{2x^2} = \lim_{x \rightarrow \infty} \frac{7x^4+7x^3}{2x^2} = \lim_{x \rightarrow \infty} \frac{7x^2+7x}{2} \rightarrow 0$, which is finite.

Thus $x = 0$ is a regular singular point and we solve the differential equation using the Frobenius Method.

The solution is of the form $y = \sum_{n=0}^{\infty} a_n x^{n+r}$ where $a_n \neq 0$.

Then, $y' = \sum_{n=0}^{\infty} (n+r) a_n x^{n+r-1}$ and $y'' = \sum_{n=0}^{\infty} (n+r)(n+r-1) a_n x^{n+r-2}$.

Substituting into the differential equation, $2x^2 \sum_{n=0}^{\infty} (n+r)(n+r-1) a_n x^{n+r-2} + 7x \sum_{n=0}^{\infty} (n+r) a_n x^{n+r-1} - 3 \sum_{n=0}^{\infty} a_n x^{n+r} = 0$.

Rearranging, $2 \sum_{n=0}^{\infty} (n+r)(n+r-1)a_n x^{n+r} + 7 \sum_{n=0}^{\infty} (n+r)a_n x^{n+r+1} + 7 \sum_{n=0}^{\infty} (n+r)a_n x^{n+r} - 3 \sum_{n=0}^{\infty} a_n x^{n+r} = 0$.

Factoring, $\sum_{n=0}^{\infty} [2(n+r)(n+r-1) + 7(n+r) - 3]a_n x^{n+r} + 7 \sum_{n=0}^{\infty} (n+r-1)a_{n-1} x^{n+r}$.

When $n = 0$, $2r(r-1) + 7r - 3 = 0 \Rightarrow 2r^2 + 5r - 3 = 0$.

By the quadratic formula, $r = \frac{-5 \pm \sqrt{5^2 - 4(2)(-3)}}{2(2)} = \frac{-5 \pm 7}{4} \Rightarrow r_1 = \frac{1}{2}, r_2 = -3$.

$r_1 - r_2 = \frac{7}{2}$, which is not an integer, so there are two independent Frobenius solutions.

By substitution, $y_1 = x^{\frac{1}{2}} \sum_{n=0}^{\infty} a_n x^n$ and $y_2 = x^{-3} \sum_{n=0}^{\infty} b_n x^n$.